## 88. Merge Sorted Array (Easy)

https://leetcode.com/problems/merge-sorted-array/

### Problem Description

Given two sorted integer arrays `nums1` and `nums`2, merge `nums2` into `nums1` as one sorted array.

The number of elements initialized in `nums1` and `nums2` are `m` and `n` respectively. You may assume that `nums1` has a size equal to `m + n` such that it has enough space to hold additional elements from `nums2`.
 

**Example 1**:
```
Input: [1,0,2,3,0,4,5,0]
Output: null
Explanation: After calling your function, the input array is modified to: [1,0,0,2,3,0,0,4]

```
### Solutions

Javascript:

```javascript
var merge = function (nums1, m, nums2, n) {
  // 设置一个指针，指针初始化指向nums1的末尾（根据#62，应该是index为 m+n-1 的位置，因为nums1的长度有可能更长）
  // 然后不断左移指针更新元素
  let current = m + n - 1;

  while (current >= 0) {
    // 没必要继续了
    if (n === 0) return;

    // 为了方便大家理解，这里代码有点赘余
    if (m < 1) {
      nums1[current--] = nums2[--n];
      continue;
    }

    if (n < 1) {
      nums1[current--] = nums1[--m];
      continue;
    }
    // 取大的填充 nums1的末尾
    // 然后更新 m 或者 n
    if (nums1[m - 1] > nums2[n - 1]) {
      nums1[current--] = nums1[--m];
    } else {
      nums1[current--] = nums2[--n];
    }
  }
};
```
```javascript
var merge = function(nums1, m, nums2, n) {
      var len = m + n;
    m--;
    n--;
    while (len--) {
        if (n < 0 || nums1[m] > nums2[n]) {
            nums1[len] = nums1[m--];
        } else {
            nums1[len] = nums2[n--];
        }
    }
};
```


Java:

```java
class Solution {
    public void merge(int[] nums1, int m, int[] nums2, int n) {
        int i=m-1, j=n-1, k=m+n-1;
        // 合并
        while(i>=0 && j>=0)
        {
            if(nums1[i] > nums2[j])
            {
                nums1[k--] = nums1[i--];
            }
            else
            {
                nums1[k--] = nums2[j--];
            }
        }
        // 合并剩余的nums2
        while(j>=0)
        {
            nums1[k--] = nums2[j--];
        }
    }
}
```
Go
```go
func merge(nums1 []int, m int, nums2 []int, n int)  {
    for p := m+n; m > 0 && n > 0; p-- {
        if nums1[m-1] <= nums2[n-1] {
            nums1[p-1] = nums2[n-1]
            n--
        } else {
            nums1[p-1] = nums1[m-1]
            m-- 
        }
    }
    for n>0 {
        nums1[n-1] = nums2[n-1]
        n--
    }
}
```
